NCML/CK/Logic/CK4Box.lean
@@ -1,0 +1,65 @@
+module
+
+public import NCML.CK.Frame.FourBox
+public import NCML.CK.Canonical
+public import NCML.CK.Soundness
+
+@[expose] public section
+
+namespace BDLogic
+
+class FourBox (L : BDLogic) where
+  fourBox {A} : (□A 🡒 □□A) ∈ L
+export FourBox (fourBox)
+
+end BDLogic
+
+instance : LogicCK4Box.FourBox := ⟨by grind⟩
+
+open ProvableBDHilbert
+
+namespace CK
+
+variable {κ : Type*} {M : Model κ}
+variable {A : BDFormula}
+
+namespace Model
+
+open CK.Frame
+
+lemma valid_of_mem_LogicCK4Box [M.FourBox] (hA : A ∈ LogicCK4Box) : M ⊧ A :=
+  valid_of_mem_logic
+    (by rintro B ⟨C, rfl⟩; exact valid_of_toFrame_valid frameValidate_FourBox_of_frame_FourBox) hA
+
+end Model
+
+variable {L : BDLogic} [L.CK]
+
+instance fourBox_canonicalModel [L.FourBox] : (canonicalModel L).FourBox where
+  fourBox {X Y Z W} MXY IYZ MZW _ := by
+    refine ⟨X.erase, W.erase, CanonicalPair.iRel_erase, ⟨?_, by simp⟩, subset_rfl⟩;
+    intro A hA;
+    have h₁ : □□A ∈ X.theory := X.theory.mdp (X.theory.subset L.fourBox) hA;
+    have h₂ : □A ∈ Y.theory := MXY.1 h₁;
+    have h₃ : □A ∈ Z.theory := IYZ h₂;
+    exact MZW.1 h₃;
+
+end CK
+
+theorem LogicCK4Box_TFAE {A : BDFormula} : List.TFAE [
+  A ∈ LogicCK4Box,
+  ∀ {κ : Type 0}, ∀ F : CK.Frame κ, [F.FourBox] → F ⊧ A,
+] := by
+  tfae_have 1 → 2 := fun h _ F _ V V_per V_fal => CK.Model.valid_of_mem_LogicCK4Box h
+  tfae_have 2 → 1 := by
+    contrapose!;
+    intro h;
+    obtain ⟨P, h₁⟩ := CK.exists_not_forces_of_not_mem h;
+    refine ⟨_, (CK.canonicalModel LogicCK4Box).toFrame, ?_⟩;
+    and_intros;
+    . infer_instance;
+    . by_contra! hF;
+      exact h₁ $ CK.Model.valid_of_toFrame_valid hF P;
+  tfae_finish
+
+end
