NCML/CK/Logic/CS4.lean
@@ -1,0 +1,57 @@
+module
+
+public import NCML.CK.CanonicalHereditary
+public import NCML.CK.Frame.CS4
+public import NCML.CK.Soundness
+
+@[expose] public section
+
+instance : LogicCS4.TBox := ⟨LogicCS4.provable_TBox⟩
+instance : LogicCS4.TDia := ⟨LogicCS4.provable_TDia⟩
+instance : LogicCS4.FourBox := ⟨LogicCS4.provable_FourBox⟩
+instance : LogicCS4.FourDia := ⟨LogicCS4.provable_FourDia⟩
+
+open ProvableBDHilbert
+open scoped BDFormulaSet BDFormulaList
+
+namespace CK
+
+variable {κ : Type*} {M : Model κ}
+variable {A : BDFormula}
+
+namespace Model
+
+open CK.Frame
+
+lemma valid_of_mem_LogicCS4 [M.T] [M.Four] (hA : A ∈ LogicCS4) : M ⊧ A :=
+  valid_of_mem_logic (by
+    rintro B (((⟨C, rfl⟩ | ⟨C, rfl⟩) | ⟨C, rfl⟩) | ⟨C, rfl⟩);
+    · exact valid_of_toFrame_valid frameValidate_TBox_of_frame_TBox;
+    · exact valid_of_toFrame_valid frameValidate_TDia_of_frame_TDia;
+    · exact valid_of_toFrame_valid frameValidate_FourBox_of_frame_FourBox;
+    · exact valid_of_toFrame_valid frameValidate_FourDia_of_frame_FourDia;
+  ) hA
+
+end Model
+
+end CK
+
+theorem LogicCS4_TFAE {A : BDFormula} : List.TFAE [
+  A ∈ LogicCS4,
+  ∀ {κ : Type 0}, ∀ F : CK.Frame κ, [F.T] → [F.Four] → F ⊧ A,
+  ∀ {κ : Type 0}, ∀ F : CK.Frame κ, [F.CS4] → F ⊧ A,
+] := by
+  tfae_have 1 → 2 := fun h _ F _ _ V V_per V_fal => CK.Model.valid_of_mem_LogicCS4 h
+  tfae_have 2 → 3 := fun h _ F _ => h F
+  tfae_have 3 → 1 := by
+    contrapose!;
+    intro h;
+    obtain ⟨X, h₁⟩ := CK.hereditary_exists_not_forces_of_not_mem h;
+    refine ⟨_, (CK.hereditaryCanonicalModel LogicCS4).toFrame, ?_⟩;
+    and_intros;
+    . infer_instance;
+    . by_contra! hF;
+      exact h₁ $ CK.Model.valid_of_toFrame_valid hF X;
+  tfae_finish
+
+end
